{
 "cells": [
  {
   "cell_type": "markdown",
   "metadata": {},
   "source": [
    "## Problem 2 ##\n",
    "\n",
    "Consider the finite discretely sampled time-series $g_{n} = g(n\\Delta)$, where $n = -N/2,..0,..N/2$ and $\\Delta$ is the sample interval. Find an expression for a **discrete, finite data window** and an expression for a **discrete finite spectral window.**"
   ]
  },
  {
   "cell_type": "markdown",
   "metadata": {},
   "source": [
    "### 2a. Derive a discrete, finite data window for *$g_{n}$*  ###\n",
    "\n",
    "*2.1.1 Express the finite discrete time series, $g_{t}^{T}$ in terms of the gate function, a sampling function, and the continuous time series.*  \n",
    "\n",
    "$g_{t}^{T} = \\prod(\\frac{t}{N\\Delta}) \\cdot III(\\frac{t}{\\Delta}) \\cdot g(t)$  \n",
    "- $\\prod(\\frac{t}{N\\Delta})$ is the gate function (boxcar), centered in time. \n",
    "\n",
    "\n",
    "- $III(\\frac{t}{\\Delta})$ is the sampling function, or shaw function \n",
    "\n",
    "\n",
    "- $g_{n} = g(t)$ is the continuous time series\n",
    "\n",
    "\n",
    "\n",
    "*2.1.2 Express finite, discrete time-series in terms of a sampling data data window, $s_{\\Delta}(t)$*  \n",
    "\n",
    "$g_{t}^{T} = \\prod(\\frac{t}{N\\Delta}) \\cdot III(\\frac{t}{\\Delta}) \\cdot g(t) \\quad$ <===> $ \\quad g_{t}^{T} = s_{\\Delta}(t) \\cdot g(t)$\n",
    "- $s_{\\Delta}(t) = \\prod(\\frac{t}{N\\Delta}) \\cdot III(\\frac{t}{\\Delta})$\n",
    "\n",
    "\n",
    "\n",
    "*2.1.3 Derive expression for discrete, finite data window*\n",
    "\n",
    "$s_{\\Delta}(t) = \\sum_{n=N/2}^{N/2}w_{n} \\delta(t - n\\Delta)$\n",
    "- $w_{n} = \\prod(\\frac{t}{N\\Delta}) = 1$, when $w_{n}$ is a boxcar.\n",
    "\n",
    "$s_{\\Delta}(t) = \\sum_{n=N/2}^{N/2} \\delta(t - n\\Delta)$\n"
   ]
  },
  {
   "cell_type": "markdown",
   "metadata": {},
   "source": [
    "### 2b: Derive a discrete, finite sampling window for *$s_{\\Delta}(t)$*  ##\n",
    "\n",
    "*2.2.1 Express $s_{\\Delta}(t)$ as $S_{\\Delta}(f)$*\n",
    "\n",
    "$S_{\\Delta}(f) = { \\int_{-\\infty}^{\\infty}} \\:s_{\\Delta}(t) \\: e^{-i2\\pi f\\Delta} dt$\n",
    "\n",
    "$S_{\\Delta}(f) = { \\int_{-\\infty}^{\\infty}} \\:\\sum_{n = -N/2}^{N/2}\\delta(n - \\Delta) \\: e^{-i2\\pi f\\Delta} dt$\n",
    "\n",
    "\n",
    "\n",
    "*2.2.2 From sifting property $S_{\\Delta}(f)$ becomes...*\n",
    "\n",
    "$S_{\\Delta}(f) = \\sum_{n = -N/2}^{N/2} \\: e^{-i2\\pi fn\\Delta}$\n",
    "\n",
    "\n",
    "\n",
    "*2.2.3 Multiply left side of equation by 1*\n",
    "\n",
    "$\\Big[S_{\\Delta}(f) = \\sum_{n = -N/2}^{N/2} \\: e^{-i2\\pi fn\\Delta}\\Big]\\frac{e^{i \\pi f \\Delta} - e^{-i \\pi f \\Delta}}{2i sin(\\pi f \\Delta)} $\n",
    "- Where  $1 = \\frac{sin(\\pi f \\Delta)}{sin(\\pi f \\Delta)} = \\frac{e^{i \\pi f \\Delta} - e^{-i \\pi f \\Delta}}{2i sin(\\pi f \\Delta)} $\n",
    "\n",
    "$ S_{\\Delta}(f) = \\sum_{n = -N/2}^{N/2} \\: \\big[e^{-i2\\pi fn\\Delta}(e^{i \\pi f \\Delta} - e^{-i \\pi f \\Delta})\\big] (\\frac{1}{2i sin(\\pi f \\Delta)})$\n",
    "\n",
    "\n",
    "*2.2.4 Use exponent properties to rearrange the two summations*\n",
    "\n",
    "$\\big(\\frac{1}{2i sin(\\pi f \\Delta)}\\big) \\:\\:S_{\\Delta}(f)=\\sum_{n = -N/2}^{N/2} e^{-i\\pi f\\Delta(2n-1)} - e^{-i \\pi f \\Delta(2n+1)}$\n",
    "\n",
    "\n",
    "\n",
    "$\\big(\\frac{1}{2i sin(\\pi f \\Delta)}\\big) \\:\\:S_{\\Delta}(f)=\\sum_{n = -N/2}^{N/2} e^{-i\\pi f\\Delta(2n-1)} - \\sum_{n = -N/2}^{N/2}e^{-i \\pi f \\Delta(2n+1)}$\n",
    "\n",
    "\n",
    "*2.2.5 Show that all terms cancel out besides $n = -N$ and $n = N$. Assume $N = 6$ and $\\frac{1}{2i sin(\\pi f \\Delta)}$ are $-i\\pi f\\Delta$ are constants *\n",
    "\n",
    "        N = 6;\n",
    "        k = 0;\n",
    "        for n = - N/2:N/2\n",
    "           k = k+1;\n",
    "           A(k) = exp(2n + 1)\n",
    "           B(k) = exp(2n - 1)\n",
    "        end\n",
    "        \n",
    "\n",
    "*2.2.6 Write $S_{\\Delta}(f)$ in terms of $n = -N$ and $n = N$*\n",
    "\n",
    "$S_{\\Delta}(f) = \\frac{e^{i\\pi fN\\Delta} \\: - \\:e^{-i\\pi fN\\Delta}}{2i sin(\\pi f \\Delta)}$\n",
    "\n",
    "\n",
    "*2.2.7 Write exponentials in terms of cosines and sines*\n",
    "\n",
    "$S_{\\Delta}(f) = \\frac{sin(\\pi f N \\Delta)}{sin(\\pi f \\Delta)}$\n",
    "- $sin(\\phi) \\: = \\: \\frac{e^{\\phi} - e^{-\\phi}}{2i}$ is an euler identity\n",
    "\n",
    "*2.2.7 Multiply by 1 and rewrite ratio in terms of sinc functions*\n",
    "\n",
    "$\\big[S_{\\Delta}(f) = \\frac{sin(\\pi f N \\Delta)}{sin(\\pi f \\Delta)}\\big]\\frac{\\pi f \\Delta}{\\pi f \\Delta}$\n",
    "\n",
    "\n",
    "$[S_{\\Delta}(f) = N_{0}\\frac{sinc(f N \\Delta)}{sinc(f \\Delta)} $\n",
    "- where $ 1 = \\frac{\\pi f \\Delta}{\\pi f \\Delta}$\n",
    "- $N_{0} =$ total number of data points \n",
    "\n",
    "\n",
    "*The above proof shows the the discrete fourier transform for a discrete, finite spectral window*\n",
    "\n",
    "$s_{\\Delta}(t) = \\sum_{n=N/2}^{N/2} \\delta(t - n\\Delta) \\quad \\supset \\quad S_{\\Delta}(f) = N_{0}\\frac{sinc(f N \\Delta)}{sinc(f \\Delta)} $\n"
   ]
  },
  {
   "cell_type": "markdown",
   "metadata": {},
   "source": [
    "## Problem 3 ##\n",
    "\n",
    "Consider the continuous time series $g(t) = cos(2\\pi f_{0}t)$."
   ]
  },
  {
   "cell_type": "markdown",
   "metadata": {},
   "source": [
    "### 3a. Derive an expression for the sample Fourier Transform $\\widehat{G}(f)$ of the finite discrete time series $g_{n} = g(n\\Delta)$, $n = -N/2,..0,..N/2$.  ###\n",
    "\n",
    "*3.1.1 Express $g_{n}$ as the sample Fourier Transfrom*\n",
    "\n",
    "$g(t) = cos(2\\pi f_{0}t)$\n",
    "\n",
    "\n",
    "$G_{n} = \\int_{-\\infty}^{\\infty}\\:S_{\\Delta}(t) \\cdot g_{n}e^{-i2\\pi ft}dt$\n",
    "- $s_{\\Delta}(t) = \\prod(\\frac{t}{N\\Delta}) \\cdot III(\\frac{t}{\\Delta})$ <===> $s_{\\Delta}(t) = \\sum_{n=N/2}^{N/2} \\delta(t - n\\Delta)$, a boxcar data window.\n",
    "- $g_{n}$ is a discretely sampled funtion.\n",
    "\n",
    "$G_{n} = \\int_{-\\infty}^{\\infty}\\:\\sum_{n=N/2}^{N/2} \\delta(t - n\\Delta)\\:cos(2\\pi f_{0}t)\\:e^{-i2\\pi ft}dt$\n",
    "\n",
    "\n",
    "*3.1.2 Apply sifting property*\n",
    "\n",
    "$G_{n} =\\sum_{n=N/2}^{N/2}\\:cos(2\\pi f_{0}n\\Delta)e^{-i2\\pi fn\\Delta}$\n",
    "\n",
    "*3.1.3 Replace cosine with exponents*\n",
    "\n",
    "$G_{n} =\\sum_{n=N/2}^{N/2}\\:\\frac{1}{2}(e^{i2\\pi f_{0}n\\Delta} + e^{-i2\\pi f_{0}n\\Delta})\\:e^{-i2\\pi fn \\Delta}$\n",
    "- where $cos(\\phi) = \\frac{1}{2}(e^{i\\phi}+e^{-i\\phi})$\n",
    "\n",
    "*3.1.4 Reduce function with exponent rules, where $e^{a}(e^{b} + e^{c})$ = $e^{a+b} + e^{a+c}$*\n",
    "\n",
    "$G_{n} =\\sum_{n=N/2}^{N/2}\\:\\frac{1}{2}e^{-i2 \\pi n\\Delta(f - f_{0})} \\:+\\: \\sum_{n=N/2}^{N/2}\\:\\frac{1}{2}e^{-i2\\pi n\\Delta(f+f_{0})}$\n",
    "\n",
    "\n",
    "*3.1.5 Multiply $G_{n}$ by 1 and rearrange by exponent rules*\n",
    "\n",
    "$G_{n} =\\sum_{n=N/2}^{N/2}\\:(\\frac{e^{-i2 \\pi n\\Delta f'}}{2})(\\frac{e^{i \\pi f' \\Delta} - e^{-i \\pi f' \\Delta}}{2i sin(\\pi f' \\Delta)}) \\:+\\: \\sum_{n=N/2}^{N/2}\\:(\\frac{e^{-i2\\pi n\\Delta(f'')}}{2})(\\frac{e^{i \\pi f'' \\Delta} - e^{-i \\pi f'' \\Delta}}{2i sin(\\pi f'' \\Delta)})$\n",
    "\n",
    "- where  $1 = \\frac{sin(\\pi f \\Delta)}{sin(\\pi f \\Delta)} = \\frac{e^{i \\pi f \\Delta} - e^{-i \\pi f \\Delta}}{2i sin(\\pi f \\Delta)} $\n",
    "\n",
    "\n",
    "- let $f^{'} = f-f_{0}$ and $f^{''} = f+f_{0}$\n",
    "\n",
    "$G_{n} =\\sum_{n=N/2}^{N/2}\\:(\\frac{e^{i2\\pi f'\\Delta(2n-1)} -e^{-i2\\pi f'\\Delta(2n+1)}}{4isin(\\pi f'\\Delta)}) \\: + \\sum_{n=N/2}^{N/2}\\:(\\frac{e^{-i2\\pi f''\\Delta(2n+1)}-e^{-i2\\pi f''\\Delta(2n-1)}}{4isin(\\pi f''\\Delta)})$\n",
    "\n",
    "*3.1.6 Similar to 2b (2.2.5), all terms except for the first positive and last negative cancel out, where $n = N_{0}$ and $n = -N_{0}$. $G_{n} =$:*\n",
    "\n",
    "$G_{n} = \\frac{1}{2}(\\frac{e^{i2\\pi f'\\Delta N_{0}} -e^{i2\\pi f'\\Delta N_{0}}}{2isin(\\pi f'\\Delta)}) + \\frac{1}{2}(\\frac{e^{-i2\\pi f''\\Delta N_{0}} -e^{-i2\\pi f''\\Delta N_{0}}}{2isin(\\pi f''\\Delta})$\n",
    "\n",
    "$G_{n} = \\frac{1}{2}(\\frac{e^{i2\\pi f'\\Delta N_{0}} -e^{i2\\pi f'\\Delta N_{0}}}{2i}\\frac{1}{sin(\\pi f'\\Delta)}) + \\frac{1}{2}(\\frac{e^{-i2\\pi f''\\Delta N_{0}} -e^{-i2\\pi f''\\Delta N_{0}}}{2i}\\frac{1}{sin(\\pi f''\\Delta})$ <===> $G_{n} = \\frac{1}{2}\\big[\\frac{sin(2\\pi f'\\Delta N_{0})}{sin(\\pi f'\\Delta)} +\\frac{sin(2\\pi f''\\Delta N_{0})}{sin(\\pi f''\\Delta)}\\big] $\n",
    "\n",
    "*3.1.7 Multiply by 1 and rewrite ratio in terms of sinc functions, as in 2b 2.1.7*\n",
    "\n",
    "$[G_{n} = \\frac{1}{2}\\big[\\frac{sin(2\\pi f'\\Delta N_{0})}{sin(\\pi f'\\Delta)}(\\frac{N_{0}\\pi f' \\Delta}{N_{0}\\pi f' \\Delta}) +\\frac{sin(2\\pi f''\\Delta N_{0})}{sin(\\pi f''\\Delta)}(\\frac{N_{0}\\pi f'' \\Delta}{N_{0}\\pi f'' \\Delta})\\big] $\n",
    "- where $1 = (\\frac{N_{0}\\pi f'' \\Delta}{N_{0}\\pi f'' \\Delta})$\n",
    "\n",
    "**$G_{n} = \\frac{N_{0}}{2}\\big[ \\frac{sinc(N_{0}\\Delta (f - f_{0})} {sinc(\\Delta (f-f_{0}))} \\:+\\:\\frac{sinc(N_{0}\\Delta (f + f_{0})} {sinc(\\Delta (f+f_{0}))}\\big]$**"
   ]
  },
  {
   "cell_type": "markdown",
   "metadata": {},
   "source": [
    "### 3b.  Show that $\\widehat{G}(f)$ is zero when $j = \\pm k$, where $f_{0} = \\frac{j}{(N+1)\\Delta}$ and $f = \\frac{k}{(N+1)\\Delta}$   ###\n",
    "\n",
    "*3.2.1 Plug $f_{0}$ and $f$ into  $\\widehat{G}(f) = \\frac{N_{0}}{2}\\big[ \\frac{sinc(N_{0}\\Delta (f - f_{0})} {sinc(\\Delta (f-f_{0}))} \\:+\\:\\frac{sinc(N_{0}\\Delta (f + f_{0})} {sinc(\\Delta (f+f_{0}))}\\big]$ *\n",
    "\n",
    "$\\widehat{G}(f) = \\frac{N_{0}}{2}\\big[ \\frac{sinc(N_{0}\\Delta (f - f_{0})} {sinc(\\Delta (f-f_{0}))} \\:+\\:\\frac{sinc(N_{0}\\Delta (f + f_{0})} {sinc(\\Delta (f+f_{0}))}\\big]$\n",
    "\n",
    "$\\widehat{G}(f) = \\frac{N_{0}}{2}\\big[ \\frac{sinc(N_{0}\\Delta(\\frac{k-j}{N_{0}\\Delta})} {sinc(\\Delta \\frac{k-j}{N_{0}\\Delta})} \\: + \\: \\frac{sinc(N_{0}\\Delta \\frac{k+j}{N_{0}\\Delta})} {sinc(\\Delta (\\frac{k+j}{N_{0}\\Delta})}\\big] $ <==> $\\widehat{G}(f) = \\frac{N_{0}}{2}\\big[ \\frac{sinc(k-j)} {sinc(\\frac{k-j}{N_{0}})} \\: + \\: \\frac{sinc(k+j)} {sinc(\\frac{k+j}{N_{0})}}\\big] $\n",
    "- where $N_{0} = N+1$\n",
    "\n",
    "*3.2.2 Convert sinc functions to sin functions *\n",
    "\n",
    "$\\widehat{G}(f) = \\frac{N_{0}}{2}\\big[ \\frac{sin(\\pi (k-j))}{sin(\\frac{\\pi (k-j)}{N_{0}})N_{0}} + \\frac{sin(\\pi (k+j))}{sin(\\frac{\\pi (k+j)}{N_{0}})N_{0}}\\big]$ <==> $\\widehat{G}(f) = \\frac{1}{2}\\big[ \\frac{sin(\\pi (k-j))}{sin(\\frac{\\pi (k-j)}{N_{0}})} + \\frac{sin(\\pi (k+j))}{sin(\\frac{\\pi (k+j)}{N_{0}})}\\big]$\n",
    "\n",
    "*3.2.3 From sine rules we know that numerator = 0 for all k and j; denominator = 0 when k = $\\pm$ j*\n",
    "\n",
    "$\\widehat{G}(f) = \\frac{1}{2}\\big[ \\frac{sin(\\pi (k-j))}{sin(\\frac{\\pi (k-j)}{N_{0}})} + \\frac{sin(\\pi (k+j))}{sin(\\frac{\\pi (k+j)}{N_{0}})}\\big]$ <==> $\\frac{0, \\: \\forall \\: k,j}{0, \\:k \\:=\\: \\pm j}$\n",
    "\n",
    "*thus...*\n",
    "\n",
    "$\\widehat{G}(f) = \\frac{1}{2}$ when $k\\: \\pm \\: j$ and $\\widehat{G}(f) = 0$, otherwise\n",
    "\n",
    "\n",
    "### 3c.  Show that $\\widehat{G}(f)$ is nonzero, where $f_{0} = \\frac{j+1/2}{(N+1)\\Delta}$ and $f = \\frac{k}{(N+1)\\Delta}$   ###\n",
    "\n",
    "*3.3.1 Following the same procedure as 3b, plug in $f_{0}$ and $f$ and change to ratio of sines*\n",
    "\n",
    "$\\widehat{G}(f) = \\frac{1}{2}\\big[ \\frac{sin(\\pi(j+1/2-k)}{sin(\\pi \\frac{j+1/2-k}{N_{0}})} \\:+ \\: \\frac{sin(\\pi(j+1/2+k)}{sin(\\pi \\frac{j+1/2+k}{N_{0}})} \\big]$\n",
    "\n",
    "*3.3.2 Following the rule of sines the numerators never equals 0 because j and k are integers and $sin(\\pi (m \\pm 1/2)) = \\pm 1$. The denominator $\\neq$ 0 because the sine never is evaluates an integer of $\\pi$ Thus .. \n",
    "\n",
    "$\\widehat{G}(f) \\neq 0, \\quad \\forall \\: j,k $\n",
    "\n",
    "### 3d.  Show that $\\widehat{G}(f)$ is nonzero, where $f_{0} = \\frac{j}{(N+1)\\Delta}$ and $f = \\frac{k+1/2}{(N+1)\\Delta}$   ###\n",
    "\n",
    "*4.1.1 Following the same logic as above, the numerators never equals 0 because j and k are integers and $sin(\\pi (m \\pm 1/2)) = \\pm 1$. The denominator $\\neq$ 0 because the sine never is evaluates an integer of $\\pi$ Thus ..\n",
    "\n",
    "$\\widehat{G}(f) \\neq 0, \\quad \\forall \\: j,k $"
   ]
  },
  {
   "cell_type": "markdown",
   "metadata": {},
   "source": [
    "## PROBLEM 5: where aliased frequencies show up ##\n",
    "\n",
    "Consider an satellite altimeters that samples sealvel at $\\Delta = 10 $ days ($\\Delta = 240$ hours). We expect the tides to dominate the sea level variations at most locations in the ocean. Find the aliased frequencies of the following tidal consituents:\n",
    "\n",
    "* $f = \\frac{1}{25.8}$ (cycles/hour) -- lunar diurnal\n",
    "* $f = \\frac{1}{12.4}$ -- lunar semidiurnal\n",
    "* $f = \\frac{1}{24.1}$ -- solar diurnal\n",
    "* $f = \\frac{1}{12}$ -- solar semidiurnal\n",
    "\n",
    "$f_{0}' = f_{0} + \\frac{n}{\\Delta} \\leq f_{n}$ <==> $n \\leq \\frac{1}{2}-f_{0}\\Delta$\n",
    "- where $f_{0}'$ = aliased frequency\n",
    "- $f_{0}$ = fundamental frequency\n",
    "- $f_{n} = \\frac{1}{2\\Delta}$ = nyquist frequency\n",
    "\n",
    "*5.1 Solve for n for above tidal constituents, where $n \\leq \\frac{1}{2}+f_{0}\\Delta$ *\n",
    "\n",
    "* $n \\leq \\frac{1}{2}+\\frac{240}{25.8}$ = 9\n",
    "\n",
    "\n",
    "* $n \\leq \\frac{1}{2}+\\frac{240}{12.4}$ = 19\n",
    "\n",
    "\n",
    "* $n \\leq \\frac{1}{2}+\\frac{240}{24.1}$ = 10\n",
    "\n",
    "\n",
    "* $n \\leq \\frac{1}{2}+\\frac{240}{12}$ = 20\n",
    "\n",
    "*5.2 Use n to solve for $f_{0}'$, the aliased frequency, where $f_{0}' = \\frac{n}{\\Delta} - f_{0}$*\n",
    "\n",
    "* $f_{0}' = \\frac{9}{240} - \\frac{1}{25.8}$ = $-0.0013$ (*lunar diurnal*)\n",
    "\n",
    "\n",
    "* $f_{0}' = \\frac{19}{240} - \\frac{1}{12.4}$ = $-0.0015$ (*lunar semidiurnal*)\n",
    "\n",
    "\n",
    "* $f_{0}' = \\frac{10}{240} - \\frac{1}{24.1}$ = $-.000017$ (*solar diurnal*)\n",
    "\n",
    "\n",
    "* $f_{0}' = \\frac{12}{240} - \\frac{1}{12}$ = $0$ (*solar semidiurnal*)"
   ]
  },
  {
   "cell_type": "markdown",
   "metadata": {},
   "source": []
  },
  {
   "cell_type": "code",
   "execution_count": null,
   "metadata": {
    "collapsed": true
   },
   "outputs": [],
   "source": []
  }
 ],
 "metadata": {
  "anaconda-cloud": {},
  "kernelspec": {
   "display_name": "Python 3",
   "language": "python",
   "name": "python3"
  },
  "language_info": {
   "codemirror_mode": {
    "name": "ipython",
    "version": 3
   },
   "file_extension": ".py",
   "mimetype": "text/x-python",
   "name": "python",
   "nbconvert_exporter": "python",
   "pygments_lexer": "ipython3",
   "version": "3.4.5"
  }
 },
 "nbformat": 4,
 "nbformat_minor": 1
}
